just need a few finishing touches
should be done by end of today

lexer.dfy
@@ -1,5 +1,8 @@
-include "types.dfy" //contains all the custom types we're using
+datatype TokenType = LEFT_PAREN | RIGHT_PAREN | DOT | MINUS | PLUS | STAR | SLASH 
+                     | UNARY_OP | BINARY_OP | VARIABLE_OP | NUMBER | EOF | TEMPSTRING | SPACE
 
+datatype Token = Pair(token_type:TokenType, token_value:string)
+datatype Result<T> = Ok(data: T) | Err(error: string)
 
 predicate validtype(token: Token){
     token.token_type==LEFT_PAREN ||
@@ -12,19 +15,112 @@ predicate validtype(token: Token){
     token.token_type==UNARY_OP ||
     token.token_type==BINARY_OP ||
     token.token_type==VARIABLE_OP ||
-    token.token_type==EOF
+    token.token_type==SPACE
+}
+predicate isWhiteSpace(ch: char){
+    ch==' '
 }
 function Flatten(tok: seq<Token>): seq<char>
-{
+/*requires forall
+ensures |Flatten(tok)|>|tok|
+ensures |tok|>=1 ==> (tok[|tok|-1].token_value==Flatten(tok)[(|Flatten(tok)|)-(|tok[|tok|-1].token_value|)..(|Flatten(tok)|)]);
+ensures forall i::0<=i<|tok| ==> exists j: nat::tok[i].token_value==Flatten(tok)[j..j+|tok[i].token_value|]*/{
     if |tok|==0 then []
     else Flatten(tok[0..|tok|-1])+tok[|tok|-1].token_value
+    
   
 }
+
+ghost predicate contains(str: seq<char>, substr: seq<char>){
+    exists i: nat:: exists l:nat :: (i+l<=|str| && substr==str[i..i+l])
+}
+
+/*lemma FlatContains(tok:seq<Token>){
+    assert |tok|>0 ==> Flatten(tok)==Flatten(tok[0..|tok|-1])+tok[|tok|-1].token_value;
+    assert exists i: nat:: exists l:nat :: (i+l<=|Flatten(tok)| && tok[|tok|-1].token_type==Flatten(tok)[i..i+l]) by {
+        var i:=
+        var l:=length()
+
+    }
+    ghost var i:=0;
+    while (i<|tok|)
+    //invariant forall j::0<=j<i ==>
+    {
+
+    }
+}
+*/
+function Spaceless(str: seq<char>): seq<char>
+{
+    if |str|==0 then []
+    else if isWhiteSpace(str[|str|-1]) then Spaceless(str[0..|str|-1])
+    else Spaceless(str[0..|str|-1])+[str[|str|-1]]
+}
+lemma SpaceAdd(ch: char,str:seq<char>)
+requires !isWhiteSpace(ch)
+ensures Spaceless(str+[ch])==Spaceless(str)+[ch];
+{
+
+}
+lemma SpaceAddTok(tokVal: seq<char>, str:seq<char>)
+requires forall i::0<=i<|tokVal| ==> !isWhiteSpace(tokVal[i])
+ensures Spaceless(str+tokVal)==Spaceless(str)+tokVal
+{
+    ghost var i:=0;
+    assert str+tokVal[0..i]==str;
+    assert Spaceless(str)+tokVal[0..i]==Spaceless(str);
+    assert Spaceless(str+tokVal[0..i])==Spaceless(str);
+    while i<|tokVal|
+    invariant i<=|tokVal|
+    invariant Spaceless(str)+tokVal[0..i]==Spaceless(str+tokVal[0..i])
+    {
+        assert !isWhiteSpace(tokVal[i]);
+        ghost var a:=str+tokVal[0..i];
+        //assert a==str+tokVal[0..i];
+        SpaceAdd(tokVal[i],a);
+        assert Spaceless(a)+[tokVal[i]]==Spaceless(a+[tokVal[i]]);
+        //assert a==str+tokVal[0..i];
+        assert a+[tokVal[i]]==str+tokVal[0..i+1];
+        assert Spaceless(str)+tokVal[0..i+1]==Spaceless(str+tokVal[0..i+1]);
+        i:=i+1;
+    }
+    assert tokVal[0..i]==tokVal;
+}
+lemma FlatAdd(tok:seq<Token>)
+    requires |tok|>=1
+    ensures Flatten(tok[0..|tok|])==Flatten(tok[0..|tok|-1])+tok[|tok|-1].token_value;
+{
+    assert tok==tok[0..|tok|];
+    assert Flatten(tok)==Flatten(tok[0..|tok|]);
+    assert Flatten(tok)==Flatten(tok[0..|tok|-1])+tok[|tok|-1].token_value;
+
+}
+
+lemma PartialFlatAdd(i: nat, tok:seq<Token>)
+    requires |tok|>=1
+    requires i<|tok|
+    ensures Flatten(tok[0..i+1])==Flatten(tok[0..i])+tok[i].token_value
+{
+    ghost var a:=tok[0..i+1];
+    FlatAdd(a);
+    assert Flatten(a)==Flatten(a[0..|a|-1])+a[|a|-1].token_value;
+    assert tok[0..i+1]==a;
+    assert tok[0..i]==a[0..|a|-1];
+}
+
 lemma Flatsame(tok: seq<Token>,tok2: seq<Token>)
 requires |tok|==|tok2|
-requires forall i :: 0<=i<|tok| ==> tok[i].token_value==tok2[i].token_value
+requires forall i :: 0<=i<|tok| ==> tok[i].token_value==tok2[i].token_value;
 ensures Flatten(tok)==Flatten(tok2)
 {
+
+}
+
+lemma FlatInclude(i: nat, tok:seq<Token>,str:seq<char>)
+requires Flatten(tok)==str
+ensures exists j : nat:: tok[i].token_value==str[j..j+|tok[i].token_value|]
+{
+
 
 }
 
@@ -43,11 +139,24 @@ predicate ValidBinary(tok: Token){
 predicate ValidVarOp(tok: Token){
     tok.token_value=="min" || tok.token_value=="max"
 }
+predicate ValidString(str: seq<char>){
+    str=="abs" ||
+    str=="sqrt" ||
+    str=="ceil" ||
+    str=="modulo" ||
+    str=="expt" ||
+    str=="min" ||
+    str=="max"
+
+}
 predicate ValidNumber(tok: Token){
     forall i::0<=i<|tok.token_value| ==>(
         (tok.token_value[i] as int >=48 && tok.token_value[i] as int  <=57)
         || tok.token_value[i]=='.'
     )
+}
+predicate ValidWhiteSpace(tok: Token){
+    tok.token_value==" " || tok.token_value=="\n" || tok.token_value=="\t"
 }
 predicate validValue(tok: Token){
     (tok.token_type==UNARY_OP ==> ValidUnary(tok)) &&
@@ -62,8 +171,8 @@ predicate validValue(tok: Token){
     (tok.token_type==RIGHT_PAREN ==> tok.token_value==")")
 }
 
-method lex(str: seq<char>) returns (tokenized: Result<seq<Token>>)
-requires forall i::0<=i<|str| ==> (
+method Lex1(str: seq<char>) returns (tokenized: Result<seq<Token>>)
+/*requires forall i::0<=i<|str| ==> (
 (str[i] as int >=48 && str[i] as int  <=57) ||
 str[i]=='+' ||
 str[i]=='-' ||
@@ -71,11 +180,11 @@ str[i]=='*' ||
 str[i]=='/' ||
 str[i]=='(' ||
 str[i]==')'
-)
+)*/
 
 
-//ensures no tempstrings
-ensures tokenized.Ok? ==> forall i:: 0<=i<|tokenized.data| ==> (validtype(tokenized.data[i]))
+
+ensures tokenized.Ok? ==> forall i:: 0<=i<|tokenized.data| ==> ((validtype(tokenized.data[i])) ||tokenized.data[i].token_type==TEMPSTRING)
 
 //ensures all tokens are valid and correct type
 ensures tokenized.Ok? ==> forall i:: 0<=i<|tokenized.data| ==> (
@@ -83,7 +192,30 @@ ensures tokenized.Ok? ==> forall i:: 0<=i<|tokenized.data| ==> (
 )
 
 //ensures all characters are represented in order in tokens
-ensures tokenized.Ok? ==> Flatten(tokenized.data)==str
+ensures tokenized.Ok? ==> Flatten(tokenized.data)==str;
+
+//ensures no false positives when returning errors
+ensures tokenized.Err? ==> (
+
+(exists i: nat:: i<|str| && !(
+    ((str[i] as int >=48 && str[i] as int  <=57) || str[i]=='.') ||
+    (str[i] as int >=97 && str[i] as int  <=122) ||
+    str[i]=='+' ||
+    str[i]=='-' ||
+    str[i]=='*' ||
+    str[i]=='/' ||
+    str[i]=='(' ||
+    str[i]==')' ||
+    (str[i]==' ' || str[i]=='\n' || str[i]=='\t')
+)
+)
+)
+/*||
+(exists i: nat ::
+!ValidString(tok[i].token_value) && forall j::0<=j<|tok[i].token_value| ==>(tok[i].token_value[j] as int >=97 && tok[i].token_value[j] as int  <=122)
+)
+*/
+
 
 {
     var i:=0;
@@ -92,7 +224,7 @@ ensures tokenized.Ok? ==> Flatten(tokenized.data)==str
     while i<|str|
     invariant forall i:: 0<=i<|tok| ==> (validtype(tok[i]) ||tok[i].token_type==TEMPSTRING)
     invariant i<=|str|
-    invariant forall i:: 0<=i<|tok| ==> validValue(tok[i])
+    invariant forall i:: 0<=i<|tok| ==> (validValue(tok[i])||tok[i].token_type==TEMPSTRING)
     invariant Flatten(tok)==str[0..i]
     {
         //numbers
@@ -107,18 +239,24 @@ ensures tokenized.Ok? ==> Flatten(tokenized.data)==str
         }
         //letters 97 to 122
         else if (str[i] as int >=97 && str[i] as int  <=122){
-            if(|tok|>=1 && tok[|tok|-1].token_type==TEMPSTRING){ //if last is number
+            if(|tok|>=1 && tok[|tok|-1].token_type==TEMPSTRING){ //if last is letter
                 tok := tok[|tok|-1 :=   //add letter
-                Pair(NUMBER,tok[|tok|-1].token_value+[str[i]])];
+                Pair(TEMPSTRING,tok[|tok|-1].token_value+[str[i]])];
+                assert(tok[|tok|-1].token_type==TEMPSTRING);
             }
             else{
                 tok:=tok + [Pair(TEMPSTRING,[str[i]])];
+                assert(tok[|tok|-1].token_type==TEMPSTRING);
             }
+            assert(tok[|tok|-1].token_type==TEMPSTRING);
+            //assert(str[i-|tok[|tok|-1].token_value|..i+1]==tok|))
         }
         //basic symbols
         else{
             if(str[i]=='+'){
                 tok:=tok + [Pair(PLUS,"+")];
+                //IDK WHY THIS LINE IN PARTICULAR HELPS THE PROVER, BUT IT DOES SO I'M KEEPING IT
+                assert Flatten(tok)==str[0..i+1];
             }
             else if(str[i]=='-'){
                tok:=tok + [Pair(MINUS,"-")];
@@ -135,26 +273,68 @@ ensures tokenized.Ok? ==> Flatten(tokenized.data)==str
             else if(str[i]==')'){
                tok:=tok + [Pair(RIGHT_PAREN,")")];
             }
+            else if(str[i]==' ' || str[i]=='\n' || str[i]=='\t'){
+                tok:=tok + [Pair(SPACE,[str[i]])];
+                assert ValidWhiteSpace(tok[|tok|-1]);
+            }
+            else{
+                assert !(
+                    ((str[i] as int >=48 && str[i] as int  <=57) || str[i]=='.') ||
+                    (str[i] as int >=97 && str[i] as int  <=122) ||
+                    str[i]=='+' ||
+                    str[i]=='-' ||
+                    str[i]=='*' ||
+                    str[i]=='/' ||
+                    str[i]=='(' ||
+                    str[i]==')' ||
+                    (str[i]==' ' || str[i]=='\n' || str[i]=='\t')
+                );
+                return Err("invalid string");
+            }  
             //tokpos:=tokpos+1;
             //num==0;
         }
+         
         assert validtype(tok[|tok|-1]) || tok[|tok|-1].token_type==TEMPSTRING;
-        assert validValue(tok[|tok|-1]);
+        assert validValue(tok[|tok|-1]) || tok[|tok|-1].token_type==TEMPSTRING;
         i:=i+1;
-        //assert Flatten(tok)==str[0..i];
+        
         //assert forall i:: 0<=i<|tok| ==> validValue(tok[i]);
     }
-    //specifying strings
-    i:=0;
-    //assert i<=|tok|;
-    assert forall i:: 0<=i<|tok| ==> (validtype(tok[i]) ||tok[i].token_type==TEMPSTRING);
-    assert Flatten(tok)==str;
+    return Ok(tok);
+
+}
+
+
+
+
+method DefineTokens (oldtok: seq<Token>, str: seq<char>) returns (tokenized: Result<seq<Token>>)
+
+//ensures no tempstrings
+ensures tokenized.Ok? ==> forall i:: 0<=i<|tokenized.data| ==> (validtype(tokenized.data[i]))
+
+//ensures all tokens are valid and correct type
+ensures tokenized.Ok? ==> forall i:: 0<=i<|tokenized.data| ==> (
+    validValue(tokenized.data[i])
+)
+
+//ensures all characters are represented in order in tokens
+ensures tokenized.Ok? ==> Flatten(tokenized.data)==str;
+requires forall i:: 0<=i<|oldtok| ==> (validtype(oldtok[i]) || oldtok[i].token_type==TEMPSTRING)
+requires forall i:: 0<=i<|oldtok| ==> (validValue(oldtok[i]) || oldtok[i].token_type==TEMPSTRING)
+requires Flatten(oldtok)==str;
+{
+    var tok:=oldtok;
+
+    
     ghost var a:=tok;
+    var i:=0;
 
     while i<|tok|
     invariant i<=|tok|
-    invariant forall j:: 0<=j<|tok| ==> validValue(tok[j])
-    invariant forall j:: 0<=j<|tok| ==> (validtype(tok[j]) ||tok[j].token_type==TEMPSTRING)
+    invariant forall j:: 0<=j<i ==> validValue(tok[j])
+    invariant forall j:: 0<=j<|tok| ==> (validtype(tok[j]) ||tok[j].token_type==TEMPSTRING);
+    invariant forall j:: 0<=j<|tok| ==> (validValue(tok[j]) ||tok[j].token_type==TEMPSTRING);
     invariant forall j:: 0<=j<i ==> ((validtype(tok[j])))
     invariant |a|==|tok|
     invariant forall j:: 0<=j<|tok| ==> a[j].token_value==tok[j].token_value
@@ -165,31 +345,72 @@ ensures tokenized.Ok? ==> Flatten(tokenized.data)==str
         if(tok[i].token_type==TEMPSTRING){ //if token is string
             
             if(ValidUnary(tok[i])){
-                
                 tok := tok[i :=
                 Pair(UNARY_OP,tok[i].token_value)];
-                
+                //assert validtype(tok[i]);
             }
             else if(ValidBinary(tok[i])){
                 tok := tok[i :=
                 Pair(BINARY_OP,tok[i].token_value)];
+                //assert validtype(tok[i]);
             }
             else if(ValidVarOp(tok[i])){
                 tok := tok[i :=
                 Pair(VARIABLE_OP,tok[i].token_value)];
+                //assert validtype(tok[i]);
             }
             else{
+                //FlatInclude(i,tok,str);
                 return Err("invalid string");
             }   
+            //assert validtype(tok[i]);
         }
         assert a[i].token_value==tok[i].token_value;
         Flatsame(tok,a);
+        assert tok[i].token_type!=TEMPSTRING;
         assert validtype(tok[i]);
         //assert tok[i].token_type==UNARY_OP ==> ValidUnary(tok[i]);
         i:=i+1;
     }
     return Ok(tok);
 }
+
+method RemoveSpaces(tok: seq<Token>) returns (spaceless: seq<Token>)
+ensures forall i:: 0<=i<|spaceless| ==> spaceless[i].token_type!=SPACE
+ensures Flatten(spaceless)==Spaceless(Flatten(tok))
+{
+    var i:=0;
+    var out: seq<Token> := [];
+    while i<|tok|
+    invariant i<=|tok|
+    invariant forall j::0<=j<|out| ==> out[j].token_type!=SPACE
+    invariant Flatten(out)==Spaceless(Flatten(tok[0..i]))
+    {
+        //assume tok[i].token_type==SPACE;
+        if tok[i].token_type!=SPACE{
+            out:=out+[tok[i]];
+            PartialFlatAdd(i,tok);
+            //FlatAdd(tok[0..i+1]);
+            assert Flatten(tok[0..i+1])==Flatten(tok[0..i])+tok[i].token_value;
+            assume tok[i].token_value=="abc";
+            SpaceAddTok(tok[i].token_value,Flatten(tok[0..i]));
+            assert Spaceless(Flatten(tok[0..i+1]))==Spaceless(Flatten(tok[0..i]))+tok[i].token_value;
+        }
+        else{
+            assume tok[i].token_value==" ";
+            PartialFlatAdd(i,tok);
+            //FlatAdd(tok[0..i+1]);
+            assert Flatten(tok[0..i+1])==Flatten(tok[0..i])+tok[i].token_value;
+            assert Spaceless(Flatten(tok[0..i+1]))==Spaceless(Flatten(tok[0..i]));
+        }
+        i:=i+1;
+    }
+    assert i==|tok|;
+    assert tok[0..|tok|]==tok;
+    return out;
+}
+
+
 
 /*match result_var
            case Ok => do something;
